formalization/thesis/Isotope/LambdaCase/Subtyping.lean
@@ -4,5 +4,6 @@ import Isotope.LambdaCase.Subtyping.Equiv
 import Isotope.LambdaCase.Subtyping.Semantics
 import Isotope.LambdaCase.Subtyping.Semantics.Named
 import Isotope.LambdaCase.Subtyping.Semantics.Categorical
+import Isotope.LambdaCase.Subtyping.Semantics.Categorical.Chosen
 import Isotope.LambdaCase.Subtyping.Semantics.Identity
 import Isotope.LambdaCase.Subtyping.Semantics.Substitution
