formalization/thesis/Isotope/LambdaSSA/Subtyping.lean
@@ -1,3 +1,5 @@
 import Isotope.LambdaSSA.Subtyping.Typing
 import Isotope.LambdaSSA.Subtyping.Semantics
+import Isotope.LambdaSSA.Subtyping.Named
+import Isotope.LambdaSSA.Subtyping.LocallyNameless
 import Isotope.LambdaSSA.Subtyping.Structural
