formalization/thesis/Isotope/LambdaSSA/Subtyping/LocallyNameless.lean
@@ -1,0 +1,2 @@
+import Isotope.LambdaSSA.Subtyping.LocallyNameless.Typing
+import Isotope.LambdaSSA.Subtyping.LocallyNameless.ToDeBruijn.Typing
