formalization/thesis/Isotope/LambdaSSA/Subtyping/Semantics.lean
@@ -1,5 +1,8 @@
 import Isotope.LambdaSSA.Subtyping.Semantics.Monadic.Term
 import Isotope.LambdaSSA.Subtyping.Semantics.Monadic.Region
+import Isotope.LambdaSSA.Subtyping.Semantics.Monadic.Renaming
 import Isotope.LambdaSSA.Subtyping.Semantics.Categorical.Term
 import Isotope.LambdaSSA.Subtyping.Semantics.Categorical.Region
 import Isotope.LambdaSSA.Subtyping.Semantics.Agreement.Term
+import Isotope.LambdaSSA.Subtyping.Semantics.Agreement.Region
+import Isotope.LambdaSSA.Subtyping.Semantics.Representation
