formalization/thesis/Isotope/LambdaSSA/Translation.lean
@@ -2,8 +2,10 @@ import Isotope.LambdaSSA.Translation.Expression
 import Isotope.LambdaSSA.Translation.FromSSA
 import Isotope.LambdaSSA.Translation.ANF.Elaboration
 import Isotope.LambdaSSA.Translation.ANF.Elaboration.Semantics
+import Isotope.LambdaSSA.Translation.ANF.Subtyping.SemanticsPreservation
 import Isotope.LambdaSSA.Translation.ANF.Elaboration.DirectElaborate
 import Isotope.LambdaSSA.Translation.ANF.ToSSA
+import Isotope.LambdaSSA.Translation.ANF.ToSSA.Subtyping.SemanticsIter
 import Isotope.LambdaSSA.Translation.Compile
 import Isotope.LambdaSSA.Translation.Compile.Semantics
 import Isotope.LambdaSSA.Translation.Compile.Subtyping
