formalization/thesis/Isotope/LambdaSeq/Subtyping/Semantics/Categorical/Chosen.lean
@@ -1,0 +1,38 @@
+import Isotope.LambdaSeq.Categorical
+
+/-! # Lambda-iter-induced categorical semantics of lambda-seq -/
+
+namespace Isotope.LambdaSeq.Subtyping.Semantics.Categorical.Chosen
+
+open CategoryTheory CategoryTheory.Limits
+open Isotope.LambdaIter.Subtyping.Semantics.Categorical
+
+universe v₁ v₂ u₁ u₂ u₃ u₄
+
+variable {V : Type u₁} {C : Type u₂}
+  [Category.{v₁} V] [Category.{v₂} C]
+  [CartesianMonoidalCategory V] [SymmetricCategory V]
+  [PremonoidalCategory C] [SymmetricPremonoidalCategory C]
+  [HasFiniteCoproducts V] [HasFiniteCoproducts C]
+  [DistributiveTensor V] [DistributivePremonoidalCategory C]
+  [Iteration C] [ElgotCategory C]
+  (J : Functor V C) [StrongElgotFreydCategory J]
+  {τ : Type u₃} [LambdaIter.TypeFormers τ] [LambdaIter.Subtyping τ]
+  (M : TypeModel τ V)
+  {ν : Type u₄} [DecidableEq ν]
+  {Φ : Type*} [LambdaIter.HasTy Φ τ] [InstructionModel J M Φ]
+
+noncomputable def denote {Γ : LambdaIter.Ctx ν τ} {n : Nat}
+    {β : LambdaSeq.LocallyNameless.BoundCtx τ n}
+    {t : LambdaSeq.LocallyNameless.Tm ν Φ n} {A : τ}
+    (h : LambdaSeq.Subtyping.LocallyNameless.HasType Φ Γ β t A) :=
+  Isotope.LambdaIter.Subtyping.Semantics.Categorical.denote J M h.embedIter
+
+theorem denote_embedIter {Γ : LambdaIter.Ctx ν τ} {n : Nat}
+    {β : LambdaSeq.LocallyNameless.BoundCtx τ n}
+    {t : LambdaSeq.LocallyNameless.Tm ν Φ n} {A : τ}
+    (h : LambdaSeq.Subtyping.LocallyNameless.HasType Φ Γ β t A) :
+    Isotope.LambdaIter.Subtyping.Semantics.Categorical.denote J M h.embedIter =
+      denote J M h := rfl
+
+end Isotope.LambdaSeq.Subtyping.Semantics.Categorical.Chosen
